update simple-nfsd proof

external/Goose/github_com/mit_pdos/goose_nfsd/simple.v
@@ -2,16 +2,30 @@
 From Perennial.goose_lang Require Import prelude.
 From Perennial.goose_lang Require Import ffi.disk_prelude.
 
+From Goose Require github_com.mit_pdos.goose_nfsd.addr.
 From Goose Require github_com.mit_pdos.goose_nfsd.buf.
 From Goose Require github_com.mit_pdos.goose_nfsd.buftxn.
 From Goose Require github_com.mit_pdos.goose_nfsd.common.
 From Goose Require github_com.mit_pdos.goose_nfsd.fh.
 From Goose Require github_com.mit_pdos.goose_nfsd.lockmap.
 From Goose Require github_com.mit_pdos.goose_nfsd.nfstypes.
-From Goose Require github_com.mit_pdos.goose_nfsd.super.
 From Goose Require github_com.mit_pdos.goose_nfsd.txn.
 From Goose Require github_com.mit_pdos.goose_nfsd.util.
 From Goose Require github_com.tchajed.marshal.
+
+(* 0super.go *)
+
+Definition block2addr: val :=
+  rec: "block2addr" "blkno" :=
+    addr.MkAddr "blkno" #0.
+
+Definition nInode: val :=
+  rec: "nInode" <> :=
+    common.INODEBLK.
+
+Definition inum2Addr: val :=
+  rec: "inum2Addr" "inum" :=
+    addr.MkAddr common.LOGSIZE ("inum" * common.INODESZ * #8).
 
 (* inode.go *)
 
@@ -41,7 +55,7 @@ Definition Decode: val :=
 
 (* Returns number of bytes read and eof *)
 Definition Inode__Read: val :=
-  rec: "Inode__Read" "ip" "btxn" "s" "offset" "bytesToRead" :=
+  rec: "Inode__Read" "ip" "btxn" "offset" "bytesToRead" :=
     (if: "offset" ≥ struct.loadF Inode.S "Size" "ip"
     then (slice.nil, #true)
     else
@@ -54,7 +68,7 @@ Definition Inode__Read: val :=
       util.DPrintf #5 (#(str"Read: off %d cnt %d
       ")) #();;
       let: "data" := ref_to (slice.T byteT) (NewSlice byteT #0) in
-      let: "buf" := buftxn.BufTxn__ReadBuf "btxn" (super.FsSuper__Block2addr "s" (struct.loadF Inode.S "Data" "ip")) common.NBITBLOCK in
+      let: "buf" := buftxn.BufTxn__ReadBuf "btxn" (block2addr (struct.loadF Inode.S "Data" "ip")) common.NBITBLOCK in
       let: "b" := ref_to uint64T #0 in
       (for: (λ: <>, ![uint64T] "b" < ![uint64T] "count"); (λ: <>, "b" <-[uint64T] ![uint64T] "b" + #1) := λ: <>,
         "data" <-[slice.T byteT] SliceAppend byteT (![slice.T byteT] "data") (SliceGet byteT (struct.loadF buf.Buf.S "Data" "buf") ("offset" + ![uint64T] "b"));;
@@ -64,15 +78,15 @@ Definition Inode__Read: val :=
       (![slice.T byteT] "data", #false)).
 
 Definition Inode__WriteInode: val :=
-  rec: "Inode__WriteInode" "ip" "btxn" "s" :=
+  rec: "Inode__WriteInode" "ip" "btxn" :=
     let: "d" := Inode__Encode "ip" in
-    buftxn.BufTxn__OverWrite "btxn" (super.FsSuper__Inum2Addr "s" (struct.loadF Inode.S "Inum" "ip")) (common.INODESZ * #8) "d";;
+    buftxn.BufTxn__OverWrite "btxn" (inum2Addr (struct.loadF Inode.S "Inum" "ip")) (common.INODESZ * #8) "d";;
     util.DPrintf #1 (#(str"WriteInode %v
     ")) #().
 
 (* Returns number of bytes written and error *)
 Definition Inode__Write: val :=
-  rec: "Inode__Write" "ip" "btxn" "s" "offset" "count" "dataBuf" :=
+  rec: "Inode__Write" "ip" "btxn" "offset" "count" "dataBuf" :=
     util.DPrintf #5 (#(str"Write: off %d cnt %d
     ")) #();;
     (if: "count" ≠ slice.len "dataBuf"
@@ -81,7 +95,7 @@ Definition Inode__Write: val :=
       (if: "offset" + "count" > disk.BlockSize
       then (#0, #false)
       else
-        let: "buffer" := buftxn.BufTxn__ReadBuf "btxn" (super.FsSuper__Block2addr "s" (struct.loadF Inode.S "Data" "ip")) common.NBITBLOCK in
+        let: "buffer" := buftxn.BufTxn__ReadBuf "btxn" (block2addr (struct.loadF Inode.S "Data" "ip")) common.NBITBLOCK in
         let: "b" := ref_to uint64T #0 in
         (for: (λ: <>, ![uint64T] "b" < "count"); (λ: <>, "b" <-[uint64T] ![uint64T] "b" + #1) := λ: <>,
           SliceSet byteT (struct.loadF buf.Buf.S "Data" "buffer") ("offset" + ![uint64T] "b") (SliceGet byteT "dataBuf" (![uint64T] "b"));;
@@ -92,14 +106,14 @@ Definition Inode__Write: val :=
         (if: "offset" + "count" > struct.loadF Inode.S "Size" "ip"
         then
           struct.storeF Inode.S "Size" "ip" ("offset" + "count");;
-          Inode__WriteInode "ip" "btxn" "s";;
+          Inode__WriteInode "ip" "btxn";;
           #()
         else #());;
         ("count", #true))).
 
 Definition ReadInode: val :=
-  rec: "ReadInode" "btxn" "s" "inum" :=
-    let: "buffer" := buftxn.BufTxn__ReadBuf "btxn" (super.FsSuper__Inum2Addr "s" "inum") (common.INODESZ * #8) in
+  rec: "ReadInode" "btxn" "inum" :=
+    let: "buffer" := buftxn.BufTxn__ReadBuf "btxn" (inum2Addr "inum") (common.INODESZ * #8) in
     let: "ip" := Decode "buffer" "inum" in
     "ip".
 
@@ -181,7 +195,6 @@ Definition Nfs__MOUNTPROC3_EXPORT: val :=
 Module Nfs.
   Definition S := struct.decl [
     "t" :: struct.ptrT txn.Txn.S;
-    "s" :: struct.ptrT super.FsSuper.S;
     "l" :: struct.ptrT lockmap.LockMap.S
   ].
 End Nfs.
@@ -190,6 +203,36 @@ Definition fh2ino: val :=
   rec: "fh2ino" "fh3" :=
     let: "fh" := fh.MakeFh "fh3" in
     struct.get fh.Fh.S "Ino" "fh".
+
+Definition rootFattr: val :=
+  rec: "rootFattr" <> :=
+    struct.mk nfstypes.Fattr3.S [
+      "Ftype" ::= nfstypes.NF3DIR;
+      "Mode" ::= #(U32 511);
+      "Nlink" ::= #(U32 1);
+      "Uid" ::= #(U32 0);
+      "Gid" ::= #(U32 0);
+      "Size" ::= #0;
+      "Used" ::= #0;
+      "Rdev" ::= struct.mk nfstypes.Specdata3.S [
+        "Specdata1" ::= #(U32 0);
+        "Specdata2" ::= #(U32 0)
+      ];
+      "Fsid" ::= #0;
+      "Fileid" ::= common.ROOTINUM;
+      "Atime" ::= struct.mk nfstypes.Nfstime3.S [
+        "Seconds" ::= #(U32 0);
+        "Nseconds" ::= #(U32 0)
+      ];
+      "Mtime" ::= struct.mk nfstypes.Nfstime3.S [
+        "Seconds" ::= #(U32 0);
+        "Nseconds" ::= #(U32 0)
+      ];
+      "Ctime" ::= struct.mk nfstypes.Nfstime3.S [
+        "Seconds" ::= #(U32 0);
+        "Nseconds" ::= #(U32 0)
+      ]
+    ].
 
 Definition Nfs__NFSPROC3_NULL: val :=
   rec: "Nfs__NFSPROC3_NULL" "nfs" :=
@@ -203,23 +246,31 @@ Definition Nfs__NFSPROC3_GETATTR: val :=
     ")) #();;
     let: "txn" := buftxn.Begin (struct.loadF Nfs.S "t" "nfs") in
     let: "inum" := fh2ino (struct.get nfstypes.GETATTR3args.S "Object" "args") in
-    (if: "inum" ≥ super.FsSuper__NInode (struct.loadF Nfs.S "s" "nfs")
+    (if: ("inum" = common.ROOTINUM)
     then
-      struct.storeF nfstypes.GETATTR3res.S "Status" "reply" nfstypes.NFS3ERR_INVAL;;
+      struct.storeF nfstypes.GETATTR3res.S "Status" "reply" nfstypes.NFS3_OK;;
+      struct.storeF nfstypes.GETATTR3resok.S "Obj_attributes" (struct.fieldRef nfstypes.GETATTR3res.S "Resok" "reply") (rootFattr #());;
       ![struct.t nfstypes.GETATTR3res.S] "reply"
     else
-      lockmap.LockMap__Acquire (struct.loadF Nfs.S "l" "nfs") "inum";;
-      let: "ip" := ReadInode "txn" (struct.loadF Nfs.S "s" "nfs") "inum" in
-      struct.storeF nfstypes.GETATTR3resok.S "Obj_attributes" (struct.fieldRef nfstypes.GETATTR3res.S "Resok" "reply") (Inode__MkFattr "ip");;
-      let: "ok" := buftxn.BufTxn__CommitWait "txn" #true in
-      (if: "ok"
-      then struct.storeF nfstypes.GETATTR3res.S "Status" "reply" nfstypes.NFS3_OK
-      else struct.storeF nfstypes.GETATTR3res.S "Status" "reply" nfstypes.NFS3ERR_SERVERFAULT);;
-      lockmap.LockMap__Release (struct.loadF Nfs.S "l" "nfs") "inum";;
-      ![struct.t nfstypes.GETATTR3res.S] "reply").
+      (if: "inum" ≥ nInode #()
+      then
+        struct.storeF nfstypes.GETATTR3res.S "Status" "reply" nfstypes.NFS3ERR_INVAL;;
+        ![struct.t nfstypes.GETATTR3res.S] "reply"
+      else
+        lockmap.LockMap__Acquire (struct.loadF Nfs.S "l" "nfs") "inum";;
+        let: "ip" := ReadInode "txn" "inum" in
+        struct.storeF nfstypes.GETATTR3resok.S "Obj_attributes" (struct.fieldRef nfstypes.GETATTR3res.S "Resok" "reply") (Inode__MkFattr "ip");;
+        let: "ok" := buftxn.BufTxn__CommitWait "txn" #true in
+        (if: "ok"
+        then struct.storeF nfstypes.GETATTR3res.S "Status" "reply" nfstypes.NFS3_OK
+        else struct.storeF nfstypes.GETATTR3res.S "Status" "reply" nfstypes.NFS3ERR_SERVERFAULT);;
+        lockmap.LockMap__Release (struct.loadF Nfs.S "l" "nfs") "inum";;
+        ![struct.t nfstypes.GETATTR3res.S] "reply")).
 
 Definition Nfs__NFSPROC3_SETATTR: val :=
   rec: "Nfs__NFSPROC3_SETATTR" "nfs" "args" :=
+    util.DPrintf #1 (#(str"NFS SetAttr %v
+    ")) #();;
     let: "reply" := ref (zero_val (struct.t nfstypes.SETATTR3res.S)) in
     struct.storeF nfstypes.SETATTR3res.S "Status" "reply" nfstypes.NFS3ERR_NOTSUPP;;
     ![struct.t nfstypes.SETATTR3res.S] "reply".
@@ -227,12 +278,38 @@ Definition Nfs__NFSPROC3_SETATTR: val :=
 (* Lookup must lock child inode to find gen number *)
 Definition Nfs__NFSPROC3_LOOKUP: val :=
   rec: "Nfs__NFSPROC3_LOOKUP" "nfs" "args" :=
+    util.DPrintf #1 (#(str"NFS Lookup %v
+    ")) #();;
     let: "reply" := ref (zero_val (struct.t nfstypes.LOOKUP3res.S)) in
-    struct.storeF nfstypes.LOOKUP3res.S "Status" "reply" nfstypes.NFS3ERR_NOTSUPP;;
-    ![struct.t nfstypes.LOOKUP3res.S] "reply".
+    let: "fn" := struct.get nfstypes.Diropargs3.S "Name" (struct.get nfstypes.LOOKUP3args.S "What" "args") in
+    let: "inum" := ref (zero_val uint64T) in
+    (if: ("fn" = #(str"a"))
+    then
+      "inum" <-[uint64T] #2;;
+      #()
+    else #());;
+    (if: ("fn" = #(str"b"))
+    then
+      "inum" <-[uint64T] #3;;
+      #()
+    else #());;
+    (if: (![uint64T] "inum" = #0) || (![uint64T] "inum" = common.ROOTINUM) || (![uint64T] "inum" ≥ nInode #())
+    then
+      struct.storeF nfstypes.LOOKUP3res.S "Status" "reply" nfstypes.NFS3ERR_NOENT;;
+      ![struct.t nfstypes.LOOKUP3res.S] "reply"
+    else
+      let: "fh" := struct.mk fh.Fh.S [
+        "Ino" ::= ![uint64T] "inum";
+        "Gen" ::= #0
+      ] in
+      struct.storeF nfstypes.LOOKUP3resok.S "Object" (struct.fieldRef nfstypes.LOOKUP3res.S "Resok" "reply") (fh.Fh__MakeFh3 "fh");;
+      struct.storeF nfstypes.LOOKUP3res.S "Status" "reply" nfstypes.NFS3_OK;;
+      ![struct.t nfstypes.LOOKUP3res.S] "reply").
 
 Definition Nfs__NFSPROC3_ACCESS: val :=
   rec: "Nfs__NFSPROC3_ACCESS" "nfs" "args" :=
+    util.DPrintf #1 (#(str"NFS Access %v
+    ")) #();;
     let: "reply" := ref (zero_val (struct.t nfstypes.ACCESS3res.S)) in
     struct.storeF nfstypes.ACCESS3res.S "Status" "reply" nfstypes.NFS3_OK;;
     struct.storeF nfstypes.ACCESS3resok.S "Access" (struct.fieldRef nfstypes.ACCESS3res.S "Resok" "reply") (nfstypes.ACCESS3_READ `or` nfstypes.ACCESS3_LOOKUP `or` nfstypes.ACCESS3_MODIFY `or` nfstypes.ACCESS3_EXTEND `or` nfstypes.ACCESS3_DELETE `or` nfstypes.ACCESS3_EXECUTE);;
@@ -245,14 +322,14 @@ Definition Nfs__NFSPROC3_READ: val :=
     ")) #();;
     let: "txn" := buftxn.Begin (struct.loadF Nfs.S "t" "nfs") in
     let: "inum" := fh2ino (struct.get nfstypes.READ3args.S "File" "args") in
-    (if: "inum" ≥ super.FsSuper__NInode (struct.loadF Nfs.S "s" "nfs")
+    (if: ("inum" = common.ROOTINUM) || ("inum" ≥ nInode #())
     then
       struct.storeF nfstypes.READ3res.S "Status" "reply" nfstypes.NFS3ERR_INVAL;;
       ![struct.t nfstypes.READ3res.S] "reply"
     else
       lockmap.LockMap__Acquire (struct.loadF Nfs.S "l" "nfs") "inum";;
-      let: "ip" := ReadInode "txn" (struct.loadF Nfs.S "s" "nfs") "inum" in
-      let: ("data", "eof") := Inode__Read "ip" "txn" (struct.loadF Nfs.S "s" "nfs") (struct.get nfstypes.READ3args.S "Offset" "args") (to_u64 (struct.get nfstypes.READ3args.S "Count" "args")) in
+      let: "ip" := ReadInode "txn" "inum" in
+      let: ("data", "eof") := Inode__Read "ip" "txn" (struct.get nfstypes.READ3args.S "Offset" "args") (to_u64 (struct.get nfstypes.READ3args.S "Count" "args")) in
       let: "ok" := buftxn.BufTxn__CommitWait "txn" #true in
       (if: "ok"
       then
@@ -271,14 +348,16 @@ Definition Nfs__NFSPROC3_WRITE: val :=
     ")) #();;
     let: "txn" := buftxn.Begin (struct.loadF Nfs.S "t" "nfs") in
     let: "inum" := fh2ino (struct.get nfstypes.WRITE3args.S "File" "args") in
-    (if: "inum" ≥ super.FsSuper__NInode (struct.loadF Nfs.S "s" "nfs")
+    util.DPrintf #1 (#(str"inum %d %d
+    ")) #();;
+    (if: ("inum" = common.ROOTINUM) || ("inum" ≥ nInode #())
     then
       struct.storeF nfstypes.WRITE3res.S "Status" "reply" nfstypes.NFS3ERR_INVAL;;
       ![struct.t nfstypes.WRITE3res.S] "reply"
     else
       lockmap.LockMap__Acquire (struct.loadF Nfs.S "l" "nfs") "inum";;
-      let: "ip" := ReadInode "txn" (struct.loadF Nfs.S "s" "nfs") "inum" in
-      let: ("count", "writeok") := Inode__Write "ip" "txn" (struct.loadF Nfs.S "s" "nfs") (struct.get nfstypes.WRITE3args.S "Offset" "args") (to_u64 (struct.get nfstypes.WRITE3args.S "Count" "args")) (struct.get nfstypes.WRITE3args.S "Data" "args") in
+      let: "ip" := ReadInode "txn" "inum" in
+      let: ("count", "writeok") := Inode__Write "ip" "txn" (struct.get nfstypes.WRITE3args.S "Offset" "args") (to_u64 (struct.get nfstypes.WRITE3args.S "Count" "args")) (struct.get nfstypes.WRITE3args.S "Data" "args") in
       (if: ~ "writeok"
       then
         lockmap.LockMap__Release (struct.loadF Nfs.S "l" "nfs") "inum";;
@@ -303,90 +382,138 @@ Definition Nfs__NFSPROC3_WRITE: val :=
 
 Definition Nfs__NFSPROC3_CREATE: val :=
   rec: "Nfs__NFSPROC3_CREATE" "nfs" "args" :=
+    util.DPrintf #1 (#(str"NFS Create %v
+    ")) #();;
     let: "reply" := ref (zero_val (struct.t nfstypes.CREATE3res.S)) in
     struct.storeF nfstypes.CREATE3res.S "Status" "reply" nfstypes.NFS3ERR_NOTSUPP;;
     ![struct.t nfstypes.CREATE3res.S] "reply".
 
 Definition Nfs__NFSPROC3_MKDIR: val :=
   rec: "Nfs__NFSPROC3_MKDIR" "nfs" "args" :=
+    util.DPrintf #1 (#(str"NFS Mkdir %v
+    ")) #();;
     let: "reply" := ref (zero_val (struct.t nfstypes.MKDIR3res.S)) in
     struct.storeF nfstypes.MKDIR3res.S "Status" "reply" nfstypes.NFS3ERR_NOTSUPP;;
     ![struct.t nfstypes.MKDIR3res.S] "reply".
 
 Definition Nfs__NFSPROC3_SYMLINK: val :=
   rec: "Nfs__NFSPROC3_SYMLINK" "nfs" "args" :=
+    util.DPrintf #1 (#(str"NFS Symlink %v
+    ")) #();;
     let: "reply" := ref (zero_val (struct.t nfstypes.SYMLINK3res.S)) in
     struct.storeF nfstypes.SYMLINK3res.S "Status" "reply" nfstypes.NFS3ERR_NOTSUPP;;
     ![struct.t nfstypes.SYMLINK3res.S] "reply".
 
 Definition Nfs__NFSPROC3_READLINK: val :=
   rec: "Nfs__NFSPROC3_READLINK" "nfs" "args" :=
+    util.DPrintf #1 (#(str"NFS Readlink %v
+    ")) #();;
     let: "reply" := ref (zero_val (struct.t nfstypes.READLINK3res.S)) in
     struct.storeF nfstypes.READLINK3res.S "Status" "reply" nfstypes.NFS3ERR_NOTSUPP;;
     ![struct.t nfstypes.READLINK3res.S] "reply".
 
 Definition Nfs__NFSPROC3_MKNOD: val :=
   rec: "Nfs__NFSPROC3_MKNOD" "nfs" "args" :=
+    util.DPrintf #1 (#(str"NFS Mknod %v
+    ")) #();;
     let: "reply" := ref (zero_val (struct.t nfstypes.MKNOD3res.S)) in
     struct.storeF nfstypes.MKNOD3res.S "Status" "reply" nfstypes.NFS3ERR_NOTSUPP;;
     ![struct.t nfstypes.MKNOD3res.S] "reply".
 
 Definition Nfs__NFSPROC3_REMOVE: val :=
   rec: "Nfs__NFSPROC3_REMOVE" "nfs" "args" :=
+    util.DPrintf #1 (#(str"NFS Remove %v
+    ")) #();;
     let: "reply" := ref (zero_val (struct.t nfstypes.REMOVE3res.S)) in
     struct.storeF nfstypes.REMOVE3res.S "Status" "reply" nfstypes.NFS3ERR_NOTSUPP;;
     ![struct.t nfstypes.REMOVE3res.S] "reply".
 
 Definition Nfs__NFSPROC3_RMDIR: val :=
   rec: "Nfs__NFSPROC3_RMDIR" "nfs" "args" :=
+    util.DPrintf #1 (#(str"NFS Rmdir %v
+    ")) #();;
     let: "reply" := ref (zero_val (struct.t nfstypes.RMDIR3res.S)) in
     struct.storeF nfstypes.RMDIR3res.S "Status" "reply" nfstypes.NFS3ERR_NOTSUPP;;
     ![struct.t nfstypes.RMDIR3res.S] "reply".
 
 Definition Nfs__NFSPROC3_RENAME: val :=
   rec: "Nfs__NFSPROC3_RENAME" "nfs" "args" :=
+    util.DPrintf #1 (#(str"NFS Rename %v
+    ")) #();;
     let: "reply" := ref (zero_val (struct.t nfstypes.RENAME3res.S)) in
     struct.storeF nfstypes.RENAME3res.S "Status" "reply" nfstypes.NFS3ERR_NOTSUPP;;
     ![struct.t nfstypes.RENAME3res.S] "reply".
 
 Definition Nfs__NFSPROC3_LINK: val :=
   rec: "Nfs__NFSPROC3_LINK" "nfs" "args" :=
+    util.DPrintf #1 (#(str"NFS Link %v
+    ")) #();;
     let: "reply" := ref (zero_val (struct.t nfstypes.LINK3res.S)) in
     struct.storeF nfstypes.LINK3res.S "Status" "reply" nfstypes.NFS3ERR_NOTSUPP;;
     ![struct.t nfstypes.LINK3res.S] "reply".
 
 Definition Nfs__NFSPROC3_READDIR: val :=
   rec: "Nfs__NFSPROC3_READDIR" "nfs" "args" :=
+    util.DPrintf #1 (#(str"NFS Readdir %v
+    ")) #();;
     let: "reply" := ref (zero_val (struct.t nfstypes.READDIR3res.S)) in
-    struct.storeF nfstypes.READDIR3res.S "Status" "reply" nfstypes.NFS3ERR_NOTSUPP;;
+    let: "e2" := struct.new nfstypes.Entry3.S [
+      "Fileid" ::= #3;
+      "Name" ::= #(str"b");
+      "Cookie" ::= #1;
+      "Nextentry" ::= slice.nil
+    ] in
+    let: "e1" := struct.new nfstypes.Entry3.S [
+      "Fileid" ::= #2;
+      "Name" ::= #(str"a");
+      "Cookie" ::= #0;
+      "Nextentry" ::= "e2"
+    ] in
+    struct.storeF nfstypes.READDIR3res.S "Status" "reply" nfstypes.NFS3_OK;;
+    struct.storeF nfstypes.READDIR3resok.S "Reply" (struct.fieldRef nfstypes.READDIR3res.S "Resok" "reply") (struct.mk nfstypes.Dirlist3.S [
+      "Entries" ::= "e1";
+      "Eof" ::= #true
+    ]);;
     ![struct.t nfstypes.READDIR3res.S] "reply".
 
 Definition Nfs__NFSPROC3_READDIRPLUS: val :=
   rec: "Nfs__NFSPROC3_READDIRPLUS" "nfs" "args" :=
+    util.DPrintf #1 (#(str"NFS Readdirplus %v
+    ")) #();;
     let: "reply" := ref (zero_val (struct.t nfstypes.READDIRPLUS3res.S)) in
     struct.storeF nfstypes.READDIRPLUS3res.S "Status" "reply" nfstypes.NFS3ERR_NOTSUPP;;
     ![struct.t nfstypes.READDIRPLUS3res.S] "reply".
 
 Definition Nfs__NFSPROC3_FSSTAT: val :=
   rec: "Nfs__NFSPROC3_FSSTAT" "nfs" "args" :=
+    util.DPrintf #1 (#(str"NFS Fsstat %v
+    ")) #();;
     let: "reply" := ref (zero_val (struct.t nfstypes.FSSTAT3res.S)) in
     struct.storeF nfstypes.FSSTAT3res.S "Status" "reply" nfstypes.NFS3ERR_NOTSUPP;;
     ![struct.t nfstypes.FSSTAT3res.S] "reply".
 
 Definition Nfs__NFSPROC3_FSINFO: val :=
   rec: "Nfs__NFSPROC3_FSINFO" "nfs" "args" :=
+    util.DPrintf #1 (#(str"NFS Fsinfo %v
+    ")) #();;
     let: "reply" := ref (zero_val (struct.t nfstypes.FSINFO3res.S)) in
-    struct.storeF nfstypes.FSINFO3res.S "Status" "reply" nfstypes.NFS3ERR_NOTSUPP;;
+    struct.storeF nfstypes.FSINFO3res.S "Status" "reply" nfstypes.NFS3_OK;;
+    struct.storeF nfstypes.FSINFO3resok.S "Wtmax" (struct.fieldRef nfstypes.FSINFO3res.S "Resok" "reply") (#(U32 4096));;
+    struct.storeF nfstypes.FSINFO3resok.S "Maxfilesize" (struct.fieldRef nfstypes.FSINFO3res.S "Resok" "reply") #4096;;
     ![struct.t nfstypes.FSINFO3res.S] "reply".
 
 Definition Nfs__NFSPROC3_PATHCONF: val :=
   rec: "Nfs__NFSPROC3_PATHCONF" "nfs" "args" :=
+    util.DPrintf #1 (#(str"NFS Pathconf %v
+    ")) #();;
     let: "reply" := ref (zero_val (struct.t nfstypes.PATHCONF3res.S)) in
     struct.storeF nfstypes.PATHCONF3res.S "Status" "reply" nfstypes.NFS3ERR_NOTSUPP;;
     ![struct.t nfstypes.PATHCONF3res.S] "reply".
 
 Definition Nfs__NFSPROC3_COMMIT: val :=
   rec: "Nfs__NFSPROC3_COMMIT" "nfs" "args" :=
+    util.DPrintf #1 (#(str"NFS Commit %v
+    ")) #();;
     let: "reply" := ref (zero_val (struct.t nfstypes.COMMIT3res.S)) in
     let: "txn" := buftxn.Begin (struct.loadF Nfs.S "t" "nfs") in
     let: "ok" := buftxn.BufTxn__CommitWait "txn" #true in
@@ -399,14 +526,10 @@ Definition Nfs__NFSPROC3_COMMIT: val :=
 
 Definition MakeNfs: val :=
   rec: "MakeNfs" "d" :=
-    let: "super" := super.MkFsSuper "d" in
-    util.DPrintf #1 (#(str"Super: %v
-    ")) #();;
     let: "txn" := txn.MkTxn "d" in
     let: "lockmap" := lockmap.MkLockMap #() in
     let: "nfs" := struct.new Nfs.S [
       "t" ::= "txn";
-      "s" ::= "super";
       "l" ::= "lockmap"
     ] in
     "nfs".
