src/program_proof/simple/simple.v
@@ -5,11 +5,11 @@ From Perennial.algebra Require Import deletable_heap liftable.
 From Perennial.Helpers Require Import Transitions.
 From Perennial.program_proof Require Import proof_prelude.
 
-From Goose.github_com.mit_pdos.goose_nfsd Require Import simple super.
-From Perennial.program_proof Require Import txn.txn_proof buftxn.buftxn_proof marshal_proof addr_proof lockmap_proof.
+From Goose.github_com.mit_pdos.goose_nfsd Require Import simple.
+From Perennial.program_proof Require Import txn.txn_proof buftxn.buftxn_proof marshal_proof addr_proof lockmap_proof addr.addr_proof.
 From Perennial.program_proof Require Import proof_prelude.
 From Perennial.program_proof Require Import disk_lib.
-From Perennial.Helpers Require Import NamedProps Map List.
+From Perennial.Helpers Require Import NamedProps Map List range_set.
 From Perennial.program_logic Require Import spec_assert.
 
 Module simple.
@@ -32,12 +32,6 @@ Record simple_names := {
 Definition LogSz : nat := 513.
 Definition InodeSz : nat := 128.
 Definition NumInodes : nat := 4096 / InodeSz.
-
-Definition is_super_mem (l: loc) : iProp Σ :=
-  "#Hsuplog" ∷ readonly (l ↦[FsSuper.S :: "nLog"] #513) ∗
-  "#Hsupbb" ∷ readonly (l ↦[FsSuper.S :: "NBlockBitmap"] #0) ∗
-  "#Hsupib" ∷ readonly (l ↦[FsSuper.S :: "NInodeBitmap"] #0) ∗
-  "#Hsupi" ∷ readonly (l ↦[FsSuper.S :: "nInodeBlk"] #1).
 
 Definition encodes_inode (len: u64) (blk: u64) data : Prop :=
   has_encoding data (EncUInt64 len :: EncUInt64 blk :: nil).
@@ -65,33 +59,41 @@ Definition is_inode_mem (l: loc) (inum: nat) (len: u64) (blk: u64) : iProp Σ :=
   l ↦[Inode.S :: "Size"] #len ∗
   l ↦[Inode.S :: "Data"] #blk.
 
-Theorem wp_Inum2Addr sup inum :
-  {{{ is_super_mem sup ∗
-      ⌜ inum < NumInodes ⌝ }}}
-    FsSuper__Inum2Addr #sup #inum
+Theorem wp_inum2Addr inum :
+  {{{ ⌜ inum < NumInodes ⌝ }}}
+    inum2Addr #inum
   {{{ RET (addr2val (inum2addr inum)); True }}}.
 Proof.
-  iIntros (Φ) "[Hsup %] HΦ".
-  iNamed "Hsup".
+  iIntros (Φ) "% HΦ".
   wp_call.
+  wp_call.
+  rewrite /addr2val /inum2addr /=.
+  rewrite /LogSz /InodeSz.
+  replace (word.add (word.divu (word.sub 4096 8) 8) 2)%Z with (U64 513) by reflexivity.
+  replace (word.mul (word.mul inum 128) 8)%Z with (U64 (inum * 128 * 8)%nat).
+  { iApply "HΦ". done. }
 
-  (* XXX goose bug: [common.INODESZ] *)
+  revert H.
+  rewrite /NumInodes /InodeSz.
+  replace (4096 `div` 128) with (32) by reflexivity.
+  intros.
+  word_cleanup.
+  admit.
 Admitted.
 
-Theorem wp_ReadInode γ inum len blk (sup btxn : loc) bufm :
-  {{{ is_super_mem sup ∗
-      is_buftxn btxn bufm γ.(simple_txn) ∗
+Theorem wp_ReadInode γ inum len blk (btxn : loc) bufm :
+  {{{ is_buftxn btxn bufm γ.(simple_txn) ∗
       is_inode_enc γ inum len blk ∗
       ⌜ inum < NumInodes ⌝ }}}
-    ReadInode #btxn #sup #inum
+    ReadInode #btxn #inum
   {{{ l, RET #l;
       is_inode_enc γ inum len blk ∗
       is_inode_mem l inum len blk }}}.
 Proof.
-  iIntros (Φ) "(#Hsup & Hbuftxn & Henc & %) HΦ".
+  iIntros (Φ) "(Hbuftxn & Henc & %) HΦ".
 
   wp_call.
-  wp_apply (wp_Inum2Addr with "[$Hsup]"); auto.
+  wp_apply (wp_inum2Addr); auto.
   replace (#(LitInt (word.mul 128 8))) with (#1024%nat) by reflexivity.
   wp_apply (wp_BufTxn__ReadBuf with "[$Hbuftxn]").
 
@@ -114,16 +116,14 @@ Definition is_inode_stable γ (inum64: u64) : iProp Σ :=
     mapsto (hG := γ.(simple_src)) inum 1%Qp state ∗
     is_inode_disk γ inum state.
 
-Definition covered_inodes : gmap u64 unit :=
-  ∅. (* Should really be 1..NumInodes maps to tt *)
+Definition covered_inodes : gset u64 :=
+  rangeSet 2 (NumInodes-2).
 
 Definition is_fs γ (nfs: loc) : iProp Σ :=
-  ∃ (txn super lm : loc),
+  ∃ (txn lm : loc),
     readonly (nfs ↦[Nfs.S :: "t"] #txn) ∗
-    readonly (nfs ↦[Nfs.S :: "s"] #super) ∗
     readonly (nfs ↦[Nfs.S :: "l"] #lm) ∗
     is_txn txn γ.(simple_txn) ∗
-    is_super_mem super ∗
     is_lockMap lm γ.(simple_lockmapghs) covered_inodes (is_inode_stable γ).
 
 End heap.
